rocq/SecTheory.v
@@ -1,0 +1,56 @@
+Require Import Basic.
+Require Import Lang.
+Require Import SecPol.
+Require Import Determinism.
+Require Import SecDef SecPol Trace.
+Require Import Grounding.
+From Coq Require Import Equality Relations RelationClasses List Compare.
+Import ListNotations.
+
+From Coq Require Import Basics Equality List Ensembles Relations RelationClasses.
+
+Module Type SecurityTheory (B : Basic) (LD : LangDefs) (TD : TraceDefs B LD) (SP : SecurityPol LD) (SD : SecurityDefs B LD TD SP) .
+  Import B LD TD SP SD.
+  Import LangNotations.
+
+  Section SilentProperties.
+      Theorem silent_indistinct : forall c m a p, sil a -> Same_set Store (atk_knowledge c m p) (atk_knowledge c m (a :: p)).
+        unfold Same_set, Included, In, atk_knowledge, deq_evt_lst.
+        intros.
+        split; split; destruct H0; trivial; destruct H1 as [st' [Ha [p' [Hprod Hdeq]]]].
+        - exists st'; split; trivial.
+          exists p'; split; trivial.
+          simpl.
+          destruct (sil_dec a); trivial.
+          contradiction.
+        - exists st'; split; trivial.
+          exists p'; split; trivial.
+          simpl in Hdeq.
+          destruct (sil_dec a); trivial.
+          contradiction.
+      Qed.
+    End SilentProperties.
+
+  Section DEqLists.
+    Theorem deq_evt_lst_refl : forall l1, 
+      deq_evt_lst l1 l1 -> deq_evt_lst l1 l1.
+      trivial.
+    Qed.
+
+    Theorem deq_evt_lst_sym : forall l1 l2, 
+      deq_evt_lst l1 l2 -> deq_evt_lst l2 l1.
+      unfold deq_evt_lst.
+      intros.
+      rewrite H.
+      reflexivity.
+    Qed.
+
+    Theorem deq_evt_lst_trans : forall l1 l2 l3,
+      deq_evt_lst l1 l2 -> deq_evt_lst l2 l3 -> deq_evt_lst l1 l3.
+      unfold deq_evt_lst.
+      intros.
+      rewrite H, H0.
+      reflexivity.
+    Qed.
+  End DEqLists.
+End SecurityTheory.
